newio/DM7.fst
@@ -21,22 +21,165 @@ let get_fun #a #w (t : pdm a w) : Pure (dm a w) (requires get_pre t) (ensures fu
 let pdm_return (a:Type) (x:a) : pdm a (hist_return x) =
  (| True, (fun _ -> dm_return _ x) |)
 
-let rec return_of (x:'a) (f:io 'a) =
+let hist_post_return (lt:trace) (x:'a) : hist_post 'a = fun lt' x' -> x == x' /\ lt == lt'
+
+(** the behavior of f can differ based on the history in iio **)
+let exists_trace (x:'a) (f:io 'a) =
+  exists lt. forall h. theta f (hist_post_return lt x) h
+
+let lemma_empty_traces_are_equal () :
+  Lemma (forall (t1 t2:trace). t1 == [] /\ t2 == [] ==> t1 == t2) = ()
+
+let emptyTrace : trace = []
+
+let lemma_theta_step cmd arg k r h klt x:
+  Lemma (requires (
+    let e = convert_call_to_event cmd arg r in
+    x `return_of` (k r) /\ x `return_of` (Call cmd arg k) /\
+    theta (k r) (hist_post_return klt x) (e::h)))
+    (ensures (
+      let e = convert_call_to_event cmd arg r in
+      theta (Call cmd arg k) (hist_post_return (e::klt) x) h)) = 
+    let e = convert_call_to_event cmd arg r in
+    let p = (hist_post_return (e::klt) x) in
+    // fun lt' x' -> x == x' /\ lt == lt'
+    calc (==) {
+      theta (Call cmd arg k) p h;
+      == { _ by (compute ())}
+      hist_bind (io_wps cmd arg) (fun r -> theta (k r)) p h;
+      == {}
+      (io_wps cmd arg) (hist_post_bind h (fun r -> theta (k r)) p) h;
+      == {_ by (compute ())}
+      io_pre cmd arg h /\ (forall r. (hist_post_bind h (fun r -> theta (k r)) p) [convert_call_to_event cmd arg r] r);
+      == {}
+      io_pre cmd arg h /\ (forall r. (fun r -> theta (k r)) r (hist_post_shift p [convert_call_to_event cmd arg r]) (List.rev [convert_call_to_event cmd arg r] @ h));
+      == {_ by (compute ())}
+      io_pre cmd arg h /\ (forall r. theta (k r) (hist_post_shift p [convert_call_to_event cmd arg r]) (convert_call_to_event cmd arg r :: h));
+    };
+    admit ()
+
+let rec lemma (x:'a) (f:io 'a) : 
+  Lemma
+    (requires (x `return_of` f))
+    (ensures (exists_trace x f)) =
   match f with
-  | Return x' -> x == x'
-  | Call cmd arg k ->
-     exists r'. return_of #'a x (k r')
+  | Return _ -> begin
+    lemma_empty_traces_are_equal ();
+
+    assert (exists lt. forall h. hist_return #event x (hist_post_return lt x) h) 
+    by (witness (`emptyTrace))
+  end 
+  | Call cmd arg k -> begin
+    assert (exists r. (x `return_of` (k r)));
+    eliminate exists r. (x `return_of` (k r)) returns (exists_trace x f) with _. begin
+      assert (x `return_of` (k r));
+      lemma x (k r);
+      assert (exists lt. (forall h. theta (k r) (hist_post_return lt x) h)) by (assumption ());
+      eliminate exists klt. (forall h. theta (k r) (hist_post_return klt x) h) returns (exists_trace x f) with _. begin
+        let e = convert_call_to_event cmd arg r in
+        introduce exists lt. (forall h. theta f (hist_post_return lt x) h) with (e::klt) and begin
+          introduce forall h. (theta f (hist_post_return (e::klt) x) h) with begin 
+            eliminate forall h'. theta (k r) (hist_post_return klt x) h' with (e::h);
+            lemma_theta_step cmd arg k r h klt x
+          end
+        end
+      end
+    end
+  end
+
+(** this is to complicated for io, but may be needed for iio: 
+let rec trace_of (lt:trace) (m:io 'a) (x:'a) =
+  match lt, m with
+  | [], Return x' -> x == x'
+  | [], Call cmd arg k -> (forall h. io_wps cmd arg (fun lt r -> lt == []) h) /\ (forall r. trace_of lt (k r) x)
+  | e::es, Call cmd arg k -> 
+          // either this is a silent call so we skip
+          ((forall h. io_wps cmd arg (fun lt r -> lt == []) h) /\ (forall r. trace_of lt (k r) x)) \/
+          // either this call has an event on the local trace
+          (let (| cmd', arg', res' |) = destruct_event e in 
+            (cmd' == cmd /\ arg == arg' /\ (trace_of es (k res') x)))
+  | _, _ -> False **)
+let rec trace_of (lt:trace) (m:io 'a) (x:'a) =
+  match lt, m with
+  | [], Return x' -> x == x'
+  | e::es, Call cmd arg k -> 
+     (let (| cmd', arg', res' |) = destruct_event e in 
+          (cmd' == cmd /\ arg == arg' /\ (trace_of es (k res') x)))
+  | _, _ -> False
+
+(** maybe worth thinking about a way to avoid using a different function: 
+let exact_2 x y = fun x' y' -> x == x' /\ y == y'
+
+let rec lemma_more_general_law m p h : 
+  Lemma 
+    (requires theta m p h) 
+    (ensures (forall lt x. theta m (exact_2 lt x) h ==> p lt x)) = () **)
+  
+let rec lemma_theta_result_implies_post m p h : 
+  Lemma 
+    (requires theta m p h) 
+    (ensures (forall x lt. trace_of lt m x ==> p lt x)) =
+  introduce forall lt x. trace_of lt m x ==> p lt x with begin
+    introduce trace_of lt m x ==> p lt x with _. begin
+      match m with
+      | Return _ -> ()
+      | Call cmd arg k -> begin
+        let e::klt = lt in
+        let (| cmd', arg', res' |) = destruct_event e in
+        lemma_theta_result_implies_post (k res') (hist_post_shift p [convert_call_to_event cmd arg res']) (convert_call_to_event cmd arg res' :: h);
+        assert (trace_of klt (k res') x);
+        assert (hist_post_shift p [convert_call_to_event cmd arg res'] klt x)
+      end
+    end
+  end
+
+let lemma_hist_bind_implies_wp2_0
+  (wp1:hist 'a) (wp2:'a -> hist 'b)
+  (m:dm 'a wp1) 
+  p h x :
+  Lemma 
+    (requires (hist_bind wp1 wp2 p h /\ x `return_of` m))
+    (ensures (exists lt. wp2 x (fun lt' r' -> p (lt @ lt') r') (List.rev lt @ h))) by (
+      ExtraTactics.blowup ();
+      bump_nth 2;
+      ExtraTactics.rewrite_lemma 9 12; 
+      let lem = ExtraTactics.get_binder 11 in
+      let bx = ExtraTactics.get_binder 7 in
+      tadmit ();
+      dump "H"
+    ) = 
+  lemma_theta_result_implies_post m (fun lt r -> wp2 r (fun lt' r' -> p (lt @ lt') r') (rev lt @ h)) h
+
+let lemma_hist_bind_implies_wp2
+  (wp1:hist 'a) (wp2:'a -> hist 'b)
+  (m:pdm 'a wp1) 
+  p h x :
+  Lemma 
+    (requires (hist_bind wp1 wp2 p h /\ x `return_of` (get_fun m)))
+    (ensures (exists lt. wp2 x p (List.rev lt @ h))) =
+  lemma_hist_bind_implies_wp2_0 wp1 wp2 (get_fun m) p h x
+
+let glue_lemma (wp:'a -> hist 'b) (pre:Type0) : Lemma
+  (requires ((forall p h x. wp x p h ==> pre) /\ 
+             (forall p h x. exists lt. wp x p (List.rev lt @ h))))
+  (ensures pre) by (
+    ExtraTactics.blowup ();
+    dump "h"
+  )= admit ()
 
 let pdm_bind (a b:Type)
   (wp1:hist a) (wp2:a -> hist b)
   (f:pdm a wp1) 
   (g:(x:a) -> pdm b (wp2 x)) :
   pdm b (hist_bind wp1 wp2) =
-  let new_pre = get_pre f /\ (forall x. x `return_of` (get_fun f) ==> get_pre (g x)) in
-  assume (forall p h. hist_bind wp1 wp2 p h ==> new_pre);
-  (| new_pre, 
+  Classical.forall_intro_3 (Classical.move_requires_3 (lemma_hist_bind_implies_wp2 wp1 wp2 f));
+  assert (forall p h x. (hist_bind wp1 wp2 p h /\ x `return_of` (get_fun f)) ==>
+            (exists lt. wp2 x p (List.rev lt @ h)));
+  assert (forall p h x. wp2 x p h ==> get_pre (g x));
+  assume ((forall p h x. exists lt. wp2 x p (List.rev lt @ h)) ==> (forall p h x. wp2 x p h));
+  assert (forall p h x. hist_bind wp1 wp2 p h /\ x `return_of` (get_fun f) ==> get_pre (g x));
+  (| (get_pre f /\ (forall x. x `return_of` (get_fun f) ==> get_pre (g x))), 
      (fun _ -> dm_bind a b wp1 wp2 (get_fun f) (fun x -> 
-       assume (x `return_of` (get_fun f));
        get_fun (g x))) |)
 
 let pdm_subcomp (a:Type) (wp1:hist a) (wp2:hist a) (f:pdm a wp1) :
